mechanization/Types/ErgoTypetoErgoCType.v
@@ -195,10 +195,9 @@ Section ErgoTypetoErgoCType.
     Definition force_brand_model_of_declarations
                (decls:list laergo_type_declaration)
       : ErgoCType.tbrand_model * list laergo_type_declaration :=
-      match brand_model_of_declarations decls with
-      | Success _ _ (s,_) => s
-      | Failure _ _ e => (tempty_brand_model, nil) (* Not used *)
-      end.
+      elift_both id
+                 (fun _ => (tempty_brand_model, nil))
+                 (brand_model_of_declarations decls).
 
   End Translate.
 
